Symbol_derive_is_derive_preds and Vec library (#3)
* trying to fmap extract and replace for symbols

* create own definition of Vec

* replace Vector and List.Vector with Vec

* proved extracts_replacesFrom_is_id

* finish proof of extracts_fmap1

* cleanup

* finish cleanup

* actually some more cleanup

Validator/Expr/Symbol.lean
@@ -31,6 +31,8 @@ import Validator.Expr.Regex
 
 namespace Symbol
 
+abbrev RegexID n := Regex (Fin n)
+
 @[reducible, simp]
 def num (r: Regex σ): Nat :=
   match r with
@@ -41,26 +43,38 @@ def num (r: Regex σ): Nat :=
   | Regex.concat r1 r2 => num r1 + num r2
   | Regex.star r1 => num r1
 
-def nums (xs: List.Vector (Regex σ) l): Nat :=
+def nums (xs: Vec (Regex σ) l): Nat :=
   match xs with
-  | ⟨[], _⟩ => 0
-  | ⟨x::xs, h⟩ => nums ⟨xs, congrArg Nat.pred h⟩ + num x
+  | Vec.nil => 0
+  | Vec.cons x xs => nums xs + num x
 
 def nums_list (xs: List (Regex σ)): Nat :=
-  nums (Vec.fromList xs)
-
-abbrev RegexID n := Regex (Fin n)
-abbrev Symbols σ l := List.Vector σ l
+  match xs with
+  | [] => 0
+  | x::xs => nums_list xs + num x
 
 def RegexID.add {n: Nat} (m: Nat) (r: RegexID n): RegexID (n + m) :=
-  Regex.map r (fun s => (Fin.mk s.val (by omega)))
+  Regex.map r (fun s => (Fin.castLE (by omega) s))
 
 def RegexID.cast (r: RegexID n) (h: n = m): RegexID m :=
   match h with
   | Eq.refl _ => r
 
-def RegexID.casts (rs: List.Vector (RegexID n) l) (h: n = m): List.Vector (RegexID m) l :=
-  List.Vector.map (fun r => RegexID.cast r h) rs
+def RegexID.castLE {n: Nat} (r: RegexID n) (h : n ≤ m): RegexID m :=
+  Regex.map r (fun s => (Fin.castLE h s))
+
+def RegexID.cast_map (r: RegexID n) (h: n = m): RegexID m :=
+  Regex.map r (fun s => Fin.castLE (by omega) s)
+
+def RegexID.casts (rs: Vec (RegexID n) l) (h: n = m): Vec (RegexID m) l :=
+  Vec.map rs (fun r => RegexID.cast r h)
+
+def RegexID.casts_rw (rs: Vec (RegexID n) l) (h: n = m): Vec (RegexID m) l := by
+  subst h
+  exact rs
+
+def RegexID.castsLE (rs: Vec (RegexID n) l) (h: n ≤ m): Vec (RegexID m) l :=
+  Vec.map rs (fun r => RegexID.castLE r h)
 
 abbrev RegexID.add_assoc (r: RegexID (n + num r1 + num r2)): RegexID (n + (num r1 + num r2)) :=
   have h : (n + num r1 + num r2) = n + (num r1 + num r2) := by
@@ -73,138 +87,21 @@ def RegexID.add_or (r: RegexID (n + num r1 + num r2)): RegexID (n + num (Regex.o
 def RegexID.add_concat (r: RegexID (n + num r1 + num r2)): RegexID (n + num (Regex.concat r1 r2)) :=
   RegexID.add_assoc r
 
-def Symbols.cast (xs: Symbols σ n) (h: n = m): Symbols σ m :=
-  match h with
-  | Eq.refl _ => xs
-
-theorem List.Vector.toList_cast_is_toList (xs: List.Vector σ n):
-  List.Vector.toList xs = List.Vector.toList (Symbols.cast xs h) := by
-  rcases xs with ⟨xs, hxs⟩
-  simp [Symbols.cast, List.Vector.toList]
-  subst h hxs
-  simp only
-
-abbrev Symbols.take {α: Type} (i: Nat) (xs: List.Vector α l) := List.Vector.take i xs
-abbrev Symbols.get {α: Type} (xs: List.Vector α l) (i: Fin l) := List.Vector.get xs i
-abbrev Symbols.nil {α: Type} := @List.Vector.nil α
-abbrev Symbols.snoc {α: Type} (xs: List.Vector α l) (x: α) := List.Vector.snoc xs x
-abbrev Symbols.cons {α: Type} (x: α) (xs: List.Vector α l) := List.Vector.cons x xs
-abbrev Symbols.set {α: Type} (v : List.Vector α l) (i : Fin l) (a : α) := List.Vector.set v i a
-abbrev Symbols.toList {α: Type} (v : List.Vector α l) := List.Vector.toList v
-
-def Symbols.add_or (xs: Symbols σ (n + num r1 + num r2)): Symbols σ (n + num (Regex.or r1 r2)) :=
+def Vec.cast_or (xs: Vec σ (n + num r1 + num r2)): Vec σ (n + num (Regex.or r1 r2)) :=
   have h : (n + num r1 + num r2) = (n + num (Regex.or r1 r2)) := by
     rw [<- Nat.add_assoc]
-  Symbols.cast xs h
+  Vec.cast xs h
 
-def Symbols.add_concat (xs: Symbols σ (n + num r1 + num r2)): Symbols σ (n + num (Regex.concat r1 r2)) :=
+def Vec.cast_concat (xs: Vec σ (n + num r1 + num r2)): Vec σ (n + num (Regex.concat r1 r2)) :=
   have h : (n + num r1 + num r2) = (n + num (Regex.concat r1 r2)) := by
     rw [<- Nat.add_assoc]
-  Symbols.cast xs h
+  Vec.cast xs h
 
-theorem Symbols.cast_rfl {xs : Symbols α n} : Symbols.cast xs rfl = xs := by
-  rcases xs with ⟨xs, rfl⟩
-  rfl
-
-theorem Symbols.take_get (xs: Symbols σ (n + m)):
-  Symbols.get (Symbols.take n xs) ⟨s, h3⟩ = Symbols.get xs ⟨s, h4⟩ := by
-  obtain ⟨xs, hxs⟩ := xs
-  simp only [List.Vector.get, List.Vector.take]
-  simp only [Fin.cast_mk, List.get_eq_getElem, List.getElem_take]
-
-theorem Symbols.cast_nil:
-  ⟨[], h1⟩ = Symbols.cast ⟨[], h3⟩ h2 := by
-  subst h3 h1
-  simp only [List.length_nil]
-  rfl
-
-theorem Symbols.cons_is_list_cons (x: σ) (xs: List.Vector σ n) (hxs: (x :: xs.val).length = n.succ):
-  ⟨List.cons x xs.val, hxs⟩ = List.Vector.cons x xs := by
-  simp only [Nat.succ_eq_add_one]
-  rfl
-
-theorem Symbols.cast_list {n m: Nat} {σ: Type} (xs: List σ) (h1: xs.length = n) (h2: m = n) (h3: xs.length = m):
-  ⟨xs, h1⟩ = Symbols.cast ⟨xs, h3⟩ h2 := by
-  apply List.Vector.eq
-  simp
-  aesop
-
-theorem Symbols.take_succ (xs: Symbols α n):
-  (
-    Symbols.take (i + 1) (Symbols.cons x xs)
-    : Symbols α (min (i + 1) (n + 1))
-  )
-  =
-  (Symbols.cast
-    (n := ((min i n) + 1))
-    (m := (min (i + 1) (n + 1)))
-    (
-      (
-        Symbols.cons x (
-          Symbols.take i xs
-        )
-      )
-      : Symbols α ((min i n) + 1)
-    )
-    (by
-      rw [Nat.min_def]
-      split_ifs
-      omega
-      omega
-    )
-  )
-  := by
-  unfold Symbols at *
-  apply List.Vector.eq
-  rw [<- List.Vector.toList_cast_is_toList]
-  rw [<- Vec.toList_take]
-  rw [<- Vec.toList_cons]
-  simp only [List.Vector.cons_val, List.take_succ_cons, List.cons.injEq, true_and]
-  rw [Vec.toList_take]
-  simp [List.Vector.toList]
-
-theorem Symbols.cast_take (xs: Symbols σ n):
-  Symbols.take n xs = Symbols.cast (n := n) (m := min n n) xs (by omega) := by
-  unfold Symbols.take
-  apply List.Vector.eq
-  generalize_proofs h
-  rw [<- List.Vector.toList_cast_is_toList]
-  rw [<- Vec.toList_take]
-  rcases xs with ⟨xs, hxs⟩
-  simp only [List.Vector.toList_mk, List.take_eq_self_iff]
-  omega
-
-theorem Symbols.cast_append_take (xs: Symbols σ n) (ys: Symbols σ m):
-  (xs ++ ys).take n = Symbols.cast (n := n) (m := min n (n + m)) xs ((by
-    omega
-  ): n = min n (n + m)) := by
-  unfold Symbols at *
-  apply List.Vector.eq
-  rw [<- List.Vector.toList_cast_is_toList]
-  rcases xs with ⟨xs, hxs⟩
-  simp only [_root_.List.Vector.toList_take, List.Vector.toList_append, List.Vector.toList_mk]
-  subst hxs
-  simp_all only [List.take_left']
-
-theorem Symbols.push_get {n: Nat} {α: Type} (xs: Symbols α n) (x: α):
-  Symbols.get (Symbols.snoc xs x) (Fin.mk n (by omega)) = x := by
-  unfold Symbols at *
-  unfold Symbols.get
-  unfold Symbols.snoc
-  rcases xs with ⟨xs, hxs⟩
-  subst hxs
-  generalize_proofs h1 h2
-  rw [List.Vector.get_eq_get_toList]
-  generalize_proofs h3
-  simp only [List.Vector.toList, List.Vector.snoc, List.Vector.cons, List.Vector.append_def]
-  simp only [Fin.cast_mk, List.get_eq_getElem, le_refl, List.getElem_append_right, tsub_self,
-    List.getElem_cons_zero]
-
-def replace (r: RegexID n) (xs: Symbols σ l) (h: n <= l): Regex σ :=
+def replace (r: RegexID n) (xs: Vec σ l) (h: n <= l): Regex σ :=
   match r with
   | Regex.emptyset => Regex.emptyset
   | Regex.emptystr => Regex.emptystr
-  | Regex.symbol s => Regex.symbol (Symbols.get xs (Fin.mk s.val (by
+  | Regex.symbol s => Regex.symbol (Vec.get xs (Fin.mk s.val (by
       cases s
       simp only
       omega
@@ -216,62 +113,198 @@ def replace (r: RegexID n) (xs: Symbols σ l) (h: n <= l): Regex σ :=
   | Regex.star r1 =>
     Regex.star (replace r1 xs h)
 
-theorem replace_cast_both (r: RegexID n) (xs: Symbols σ n) (h: n = l):
-  replace r xs (by omega) = replace (RegexID.cast r h) (Symbols.cast xs h) (by omega) := by
-  subst h
-  simp only [Symbols.cast_rfl]
+def replaceFrom (r: RegexID n) (xs: Vec σ n): Regex σ :=
+  replace r xs (le_refl n)
+
+def extract (r: Regex σ) (acc: Vec σ n): RegexID (n + num r) × Vec σ (n + num r) :=
+  match r with
+  | Regex.emptyset => (Regex.emptyset, acc)
+  | Regex.emptystr => (Regex.emptystr, acc)
+  | Regex.symbol s => (Regex.symbol (Fin.mk n (by
+      simp only [num]
+      omega
+    )), Vec.snoc acc s)
+  | Regex.or r1 r2 =>
+    let (er1, acc1) := extract r1 acc
+    let (er2, acc2) := extract r2 acc1
+    (Regex.or (RegexID.add_or (RegexID.add (num r2) er1)) (RegexID.add_or er2), Vec.cast_or acc2)
+  | Regex.concat r1 r2 =>
+    let (er1, acc1) := extract r1 acc
+    let (er2, acc2) := extract r2 acc1
+    (Regex.concat (RegexID.add_concat (RegexID.add (num r2) er1)) (RegexID.add_concat er2), Vec.cast_concat acc2)
+  | Regex.star r1 =>
+    let (er1, acc1) := extract r1 acc
+    (Regex.star er1, acc1)
+
+def extractFrom (r: Regex σ): RegexID (num r) × Vec σ (num r) :=
+  match extract r Vec.nil with
+  | (r', xs) => (RegexID.cast r' (by omega), Vec.cast xs (by omega))
+
+def derive {σ: Type} {α: Type} (p: σ -> α -> Bool) (r: Regex σ) (a: α): Regex σ :=
+  Regex.derive2
+    (replaceFrom
+      (extractFrom r).1
+      (Vec.map
+        (extractFrom r).2
+        (fun s => (s, p s a))
+      )
+    )
+
+def derive' {σ: Type} {α: Type} (p: σ -> α -> Bool) (r: Regex σ) (a: α): Regex σ :=
+  let (r', symbols): (RegexID (num r) × Vec σ (num r)) := extractFrom r
+  let pred_results: Vec Bool (num r) := Vec.map symbols (fun s => p s a)
+  let replaces: Vec (σ × Bool) (num r) := Vec.zip symbols pred_results
+  let replaced: Regex (σ × Bool) := replaceFrom r' replaces
+  Regex.derive2 replaced
+
+def extracts (xs: Vec (Regex σ) nregex) (acc: Vec σ nacc):
+  (Vec (RegexID (nacc + nums xs)) nregex) × (Vec σ (nacc + nums xs)) :=
+  match xs with
+  | Vec.nil =>
+    ( Vec.nil, acc )
+  | @Vec.cons _ nregex x xs =>
+    let (regexid, acc1) := Symbol.extract x acc
+    let (regexids, accs) := extracts xs acc1
+    let regexid': RegexID (nacc + nums (Vec.cons x xs)) :=
+      RegexID.cast (RegexID.add (nums xs) regexid) (by simp only [nums]; ac_rfl)
+    let regexesids' : Vec (RegexID (nacc + nums (Vec.cons x xs))) nregex :=
+      RegexID.casts regexids (by simp only [nums]; ac_rfl)
+    let regexidcons: Vec (RegexID (nacc + nums (Vec.cons x xs))) (nregex + 1) :=
+      Vec.cast (Vec.cons regexid' regexesids') (by simp only)
+    let accs' : (Vec σ (nacc + nums (Vec.cons x xs))) :=
+      Vec.cast accs (by simp only [nums]; ac_rfl)
+    (regexidcons, accs')
+
+def extractsFrom (xs: Vec (Regex σ) nregex):
+  (Vec (RegexID (nums xs)) nregex) × (Vec σ (nums xs)) :=
+  let (xs0, symbols0) := extracts xs Vec.nil
+  let symbols': Vec σ (nums xs) := Vec.cast symbols0 (by ac_rfl)
+  let xs': Vec (RegexID (nums xs)) nregex := RegexID.casts xs0 (by ac_rfl)
+  (xs', symbols')
+
+def replacesFrom (rs: Vec (RegexID n) l) (xs: Vec σ n): Vec (Regex σ) l :=
+  Vec.map rs (fun r => replaceFrom r xs)
+
+def derives {σ: Type} {α: Type} (p: σ -> α -> Bool) (rs: Vec (Regex σ) l) (a: α): Vec (Regex σ) l :=
+  let (rs', symbols): (Vec (RegexID (nums rs)) l × Vec σ (nums rs)) := Symbol.extractsFrom rs
+  let pred_results: Vec Bool (nums rs) := Vec.map symbols (fun s => p s a)
+  let replaces: Vec (σ × Bool) (nums rs) := Vec.zip symbols pred_results
+  let replaced: Vec (Regex (σ × Bool)) l := replacesFrom rs' replaces
+  Regex.derives2 replaced
+
+def leave
+  (rs: Vec (Regex σ) l)
+  (ps: Vec Bool (Symbol.nums rs))
+  : (Vec (Regex σ) l) :=
+  let replaces: Vec (σ × Bool) (nums rs) := Vec.zip (Symbol.extractsFrom rs).2 ps
+  let replaced: Vec (Regex (σ × Bool)) l := replacesFrom (Symbol.extractsFrom rs).1 replaces
+  Regex.derives2 replaced
+
+def enter (rs: Vec (Regex σ) l): Vec σ (nums rs) :=
+  let (_, symbols): (Vec (RegexID (nums rs)) l × Vec σ (nums rs)) := Symbol.extractsFrom rs
+  symbols
+
+-- derives_preds unlike derives takes a predicate that works out the full vector of predicates.
+-- This gives the predicate control over the evaluation order of α, for example α is a tree, we can first evaluate the same label, before traversing down.
+def derives_preds {σ: Type} {α: Type}
+  (ps: {n: Nat} -> Vec σ n -> α -> Vec Bool n) (rs: Vec (Regex σ) l) (a: α): Vec (Regex σ) l :=
+  let symbols: Vec σ (nums rs) := enter rs
+  let pred_results: Vec Bool (nums rs) := ps symbols a
+  leave rs pred_results
+
+theorem nums_nil {σ: Type}:
+  nums (@Vec.nil (Regex σ)) = 0 := by
+  unfold nums
   rfl
 
-theorem replace_cast_symbols (r: RegexID n) (xs: Symbols σ n) (h: n = l):
-  replace r xs (by omega) = replace r (Symbols.cast xs h) (by omega) := by
+theorem nums_is_nums_list (xs: Vec (Regex σ) l):
+  nums xs = nums_list xs.toList := by
+  induction xs with
+  | nil =>
+    simp only [nums, Vec.toList, nums_list]
+  | cons x xs ih =>
+    simp only [nums, Vec.toList, nums_list]
+    rw [ih]
+
+theorem RegexID.cast_rfl (r: RegexID n): RegexID.cast r rfl = r := by
+  rfl
+
+theorem RegexID.cast_rfl' (r: RegexID n) (h: n = n): RegexID.cast r h = r := by
+  rfl
+
+theorem RegexID.cast_map_rfl (r: RegexID n): RegexID.cast_map r rfl = r := by
+  unfold RegexID.cast_map
+  simp only [Fin.castLE_refl]
+  rw [Regex.map_id]
+
+theorem RegexID.cast_is_cast_map (r: RegexID n) (h: n = m):
+  RegexID.cast r h = RegexID.cast_map r h := by
   subst h
-  simp only [Symbols.cast_rfl]
+  rw [RegexID.cast_rfl]
+  rw [RegexID.cast_map_rfl]
+
+theorem replace_cast_both (r: RegexID n) (xs: Vec σ n) (h: n = l):
+  replace r xs (by omega) = replace (RegexID.cast r h) (Vec.cast xs h) (by omega) := by
+  subst h
+  simp only [Vec.cast_rfl]
+  rfl
+
+theorem replaceFrom_cast_both (r: RegexID n) (xs: Vec σ n) (h: n = l):
+  replaceFrom r xs = replaceFrom (RegexID.cast r h) (Vec.cast xs h) := by
+  unfold replaceFrom
+  rw [replace_cast_both]
+
+theorem replace_cast_symbols (r: RegexID n) (xs: Vec σ n) (h: n = l):
+  replace r xs (by omega) = replace r (Vec.cast xs h) (by omega) := by
+  subst h
+  simp only [Vec.cast_rfl]
 
 theorem replace_nil_is_map_id (r: Regex (Fin 0)):
-  replace r List.Vector.nil (by simp) = Regex.map r id := by
+  replace r Vec.nil (by simp) = Regex.map r id := by
   induction r with
   | emptyset =>
-    simp [replace, Regex.map]
+    simp only [replace, Regex.map]
   | emptystr =>
-    simp [replace, Regex.map]
+    simp only [replace, Regex.map]
   | symbol s =>
     nomatch s
   | or r1 r2 ih1 ih2 =>
-    simp [replace, Regex.map]
+    simp only [replace, Regex.map, Regex.or.injEq]
     rw [ih1]
     rw [ih2]
     apply And.intro rfl rfl
   | concat r1 r2 ih1 ih2 =>
-    simp [replace, Regex.map]
+    simp only [replace, Regex.map, Regex.concat.injEq]
     rw [ih1]
     rw [ih2]
     apply And.intro rfl rfl
   | star r1 ih1 =>
-    simp [replace, Regex.map]
+    simp only [replace, Regex.map]
     rw [ih1]
 
-theorem replace_take (r: RegexID n) (xs: Symbols σ (n + l)):
-  replace r (Symbols.take n xs) (by omega) = replace r xs (by omega):= by
+theorem replace_take (r: RegexID n) (xs: Vec σ (n + l)):
+  replace r (Vec.take n xs) (by omega) = replace r xs (by omega):= by
   induction r with
   | emptyset =>
-    simp [replace]
+    simp only [replace]
   | emptystr =>
-    simp [replace]
+    simp only [replace]
   | symbol s =>
     generalize_proofs h1 h2 at *
     simp only [replace]
     obtain ⟨s, hs⟩ := s
     simp only [Regex.symbol.injEq]
     generalize_proofs h3 h4
-    rw [Symbols.take_get]
+    rw [Vec.take_get]
+    omega
   | or r1 r2 ih1 ih2 =>
-    simp [replace]
+    simp only [replace, Regex.or.injEq]
     generalize_proofs h1 h2 at *
     rw [<- ih1]
     rw [<- ih2]
     apply And.intro rfl rfl
   | concat r1 r2 ih1 ih2 =>
-    simp [replace]
+    simp only [replace, Regex.concat.injEq]
     generalize_proofs h1 h2 at *
     rw [<- ih1]
     rw [<- ih2]
@@ -281,200 +314,165 @@ theorem replace_take (r: RegexID n) (xs: Symbols σ (n + l)):
     generalize_proofs h1 at *
     rw [<- ih1]
 
-theorem replace_regexid_add (r: RegexID n) (xs: List.Vector σ (n + l)):
+theorem replace_regexid_add (r: RegexID n) (xs: Vec σ (n + l)):
   replace r xs (by omega) = replace (RegexID.add l r) xs (by omega):= by
   generalize_proofs h1 h2
-  rcases xs with ⟨xs, hxs⟩
   induction r with
   | emptyset =>
-    simp [replace, RegexID.add, Regex.map]
+    simp only [replace, RegexID.add, Regex.map]
   | emptystr =>
-    simp [replace, RegexID.add, Regex.map]
+    simp only [replace, RegexID.add, Regex.map]
   | symbol s =>
     generalize_proofs h1 h2 at *
-    simp [replace, RegexID.add, Regex.map]
+    simp only [replace, RegexID.add, Regex.map, Fin.coe_castLE]
   | or r1 r2 ih1 ih2 =>
-    simp [replace, RegexID.add, Regex.map]
+    simp only [replace, RegexID.add, Regex.map, Regex.or.injEq]
     generalize_proofs h1 h2 at *
     rw [ih1]
     rw [ih2]
     apply And.intro rfl rfl
   | concat r1 r2 ih1 ih2 =>
-    simp [replace, RegexID.add, Regex.map]
+    simp only [replace, RegexID.add, Regex.map, Regex.concat.injEq]
     generalize_proofs h1 h2 at *
     rw [ih1]
     rw [ih2]
     apply And.intro rfl rfl
   | star r1 ih1 =>
-    simp [replace, RegexID.add, Regex.map]
+    simp only [replace, RegexID.add, Regex.map, Regex.star.injEq]
     generalize_proofs h1 h2 at *
     rw [ih1]
     rfl
 
-def extract (r: Regex σ) (acc: Symbols σ n): RegexID (n + num r) × Symbols σ (n + num r) :=
-  match r with
-  | Regex.emptyset => (Regex.emptyset, acc)
-  | Regex.emptystr => (Regex.emptystr, acc)
-  | Regex.symbol s => (Regex.symbol (Fin.mk n (by
-      simp only [num]
-      omega
-    )), Symbols.snoc acc s)
-  | Regex.or r1 r2 =>
-    let (er1, acc1) := extract r1 acc
-    let (er2, acc2) := extract r2 acc1
-    (Regex.or (RegexID.add_or (RegexID.add (num r2) er1)) (RegexID.add_or er2), Symbols.add_or acc2)
-  | Regex.concat r1 r2 =>
-    let (er1, acc1) := extract r1 acc
-    let (er2, acc2) := extract r2 acc1
-    (Regex.concat (RegexID.add_concat (RegexID.add (num r2) er1)) (RegexID.add_concat er2), Symbols.add_concat acc2)
-  | Regex.star r1 =>
-    let (er1, acc1) := extract r1 acc
-    (Regex.star er1, acc1)
-
-theorem extract_append_toList (acc: Symbols σ n) (r: Regex σ):
-  List.Vector.toList (extract r acc).2 = List.Vector.toList (acc ++ (extract r Symbols.nil).2) := by
+theorem extract_append_toList (acc: Vec σ n) (r: Regex σ):
+  Vec.toList (extract r acc).2 = Vec.toList (Vec.append acc (extract r Vec.nil).2) := by
   induction r generalizing acc n  with
   | emptyset =>
-    simp only [num, Nat.add_zero, extract, List.Vector.append_nil]
+    simp only [num, Nat.add_zero, extract, Vec.append_nil, Vec.cast_toList]
   | emptystr =>
-    simp only [num, Nat.add_zero, extract, List.Vector.append_nil]
+    simp only [num, Nat.add_zero, extract, Vec.append_nil, Vec.cast_toList]
   | symbol s =>
-    simp only [extract]
-    rfl
+    simp only [extract, Vec.snoc]
+    rw [Vec.snoc_append]
   | or r1 r2 ih1 ih2 =>
     simp only [extract]
-    rw [Symbols.add_or]
+    rw [Vec.cast_or]
     generalize_proofs h1 h2 h3
-    rw [Symbols.add_or]
+    rw [Vec.cast_or]
     generalize_proofs h4
-    rw [List.Vector.toList_append]
-    rw [<- List.Vector.toList_cast_is_toList]
-    rw [<- List.Vector.toList_cast_is_toList]
+    rw [Vec.toList_append]
+    rw [Vec.cast_toList]
+    rw [Vec.cast_toList]
     rw [ih2]
-    rw [List.Vector.toList_append]
+    rw [Vec.toList_append]
     rw [ih1]
-    rw [List.Vector.toList_append]
+    rw [Vec.toList_append]
     nth_rewrite 2 [ih2]
-    rw [List.Vector.toList_append]
+    rw [Vec.toList_append]
     ac_rfl
   | concat r1 r2 ih1 ih2 =>
     simp only [extract]
-    rw [Symbols.add_concat]
+    rw [Vec.cast_concat]
     generalize_proofs h1 h2 h3
-    rw [Symbols.add_concat]
+    rw [Vec.cast_concat]
     generalize_proofs h4
-    rw [List.Vector.toList_append]
-    rw [<- List.Vector.toList_cast_is_toList]
-    rw [<- List.Vector.toList_cast_is_toList]
+    rw [Vec.toList_append]
+    rw [Vec.cast_toList]
+    rw [Vec.cast_toList]
     rw [ih2]
-    rw [List.Vector.toList_append]
+    rw [Vec.toList_append]
     rw [ih1]
-    rw [List.Vector.toList_append]
+    rw [Vec.toList_append]
     nth_rewrite 2 [ih2]
-    rw [List.Vector.toList_append]
+    rw [Vec.toList_append]
     ac_rfl
   | star r1 ih1 =>
     simp only [extract]
     rw [ih1]
 
-theorem extract_append (acc: Symbols σ l) (r: Regex σ):
-  (extract r acc).2 = Symbols.cast (acc ++ (extract r Symbols.nil).2) (by omega) := by
-  apply List.Vector.eq
+theorem extract_append (acc: Vec σ l) (r: Regex σ):
+  (extract r acc).2 = Vec.cast (Vec.append acc (extract r Vec.nil).2) (by omega) := by
+  apply Vec.eq
   rw [extract_append_toList]
-  rw [<- List.Vector.toList_cast_is_toList]
+  rw [<- Vec.cast_toList]
 
-theorem extract_take_toList (acc: Symbols σ l):
-  (List.Vector.toList
-    (List.Vector.take
+theorem extract_take_toList (acc: Vec σ l):
+  (Vec.toList
+    (Vec.take
       (l + num r1)
       (extract r2
       (extract r1 acc).2).2
     )
   )
   =
-  (List.Vector.toList (extract r1 acc).2) := by
+  (Vec.toList (extract r1 acc).2) := by
   rw [<- Vec.toList_take]
-  rw [<- List.Vector.toList]
   rw [extract_append_toList]
-  rw [List.Vector.toList_append]
-  rw [List.Vector.toList]
-  generalize he: (extract r1 acc).2 = her
-  obtain ⟨her, hher⟩ := her
-  simp only
-  simp_all only [List.take_left']
+  rw [Vec.toList_append]
+  rw [List.take_left']
+  rw [Vec.toList_length]
 
-theorem extract_take (acc: Symbols σ l):
-  (List.Vector.take
+theorem extract_take (acc: Vec σ l):
+  (Vec.take
     (l + num r1)
     (extract r2
       (extract r1 acc).2).2
   )
   =
-    Symbols.cast
+    Vec.cast
     (extract r1 acc).2
     (by omega) := by
-  apply List.Vector.eq
+  apply Vec.eq
   rw [extract_take_toList]
-  rw [<- List.Vector.toList_cast_is_toList]
+  rw [<- Vec.cast_toList]
 
-theorem toList_fmap:
-  (List.Vector.map f xs).toList = List.map f (xs.toList) := by
-  simp_all only [List.Vector.toList_map]
-
-theorem extract_take_toList_fmap (acc: Symbols σ l):
-  (List.Vector.toList
-    (List.Vector.take
+theorem extract_take_toList_fmap (acc: Vec σ l):
+  (Vec.toList
+    (Vec.take
       (l + num r1)
-      (List.Vector.map
-        f
+      (Vec.map
         (extract r2
         (extract r1 acc).2).2
+        f
       )
     )
   )
   =
-  (List.Vector.toList
-    (List.Vector.map
-      f
+  (Vec.toList
+    (Vec.map
       (extract r1 acc).2
+      f
     )
   ) := by
   rw [<- Vec.toList_take]
-  rw [<- List.Vector.toList]
-  rw [toList_fmap]
+  rw [Vec.map_toList]
   rw [extract_append_toList]
-  rw [List.Vector.toList_append]
-  rw [List.Vector.toList]
-  generalize he: (extract r1 acc).2 = her
-  obtain ⟨her, hher⟩ := her
-  simp only
-  simp_all only [List.map_append, List.length_map, List.take_left', List.Vector.toList_map,
-    List.Vector.toList_mk]
+  rw [Vec.toList_append]
+  simp_all only [List.map_append, Vec.toList_map]
+  rw [List.take_left']
+  rw [<- Vec.map_toList]
+  rw [Vec.toList_length]
 
-theorem extract_take_fmap (acc: Symbols α l) (f: α -> β):
-  (List.Vector.take
+theorem extract_take_fmap (acc: Vec α l) (f: α -> β):
+  (Vec.take
     (l + num r1)
-    (List.Vector.map
-      f
+    (Vec.map
       (extract r2
         (extract r1 acc).2).2
+      f
     )
   )
   =
-    Symbols.cast
-    (List.Vector.map
-      f
+    Vec.cast
+    (Vec.map
       (extract r1 acc).2
+      f
     )
     (by omega) := by
-  apply List.Vector.eq
+  apply Vec.eq
   rw [extract_take_toList_fmap]
-  rw [<- List.Vector.toList_cast_is_toList]
+  rw [<- Vec.cast_toList]
 
-def replaceFrom (r: RegexID n) (xs: Symbols σ n): Regex σ :=
-  replace r xs (le_refl n)
-
-theorem extract_replaceFrom_is_id (r: Regex σ) (acc: Symbols σ l):
+theorem extract_replaceFrom_is_id (r: Regex σ) (acc: Vec σ l):
   r = replaceFrom (extract r acc).1 (extract r acc).2 := by
   simp only [replaceFrom]
   generalize_proofs hr
@@ -489,7 +487,7 @@ theorem extract_replaceFrom_is_id (r: Regex σ) (acc: Symbols σ l):
   | symbol s =>
     intro n acc hr
     simp only [replace, extract]
-    rw [Symbols.push_get]
+    rw [Vec.snoc_get]
   | or r1 r2 ih1 ih2 =>
     intro n acc hr
     simp only [extract]
@@ -498,17 +496,16 @@ theorem extract_replaceFrom_is_id (r: Regex σ) (acc: Symbols σ l):
       r1 =
         (replace
           (RegexID.add_or (RegexID.add (num r2) (extract r1 acc).1))
-          (Symbols.add_or (extract r2 (extract r1 acc).2).2)
+          (Vec.cast_or (extract r2 (extract r1 acc).2).2)
           hr
         ) := by
       clear ih2
       rw [RegexID.add_or]
-      rw [Symbols.add_or]
+      rw [Vec.cast_or]
       rw [<- replace_cast_both]
       rw [<- replace_regexid_add]
       rw [<- replace_take]
       generalize_proofs h1
-      unfold Symbols.take
       rw [extract_take]
       generalize_proofs h1 h2
       nth_rewrite 1 [ih1 acc]
@@ -518,7 +515,7 @@ theorem extract_replaceFrom_is_id (r: Regex σ) (acc: Symbols σ l):
     clear ih1
     congr
     rw [RegexID.add_or]
-    rw [Symbols.add_or]
+    rw [Vec.cast_or]
     rw [<- replace_cast_both]
     rw [<- ih2 ((extract r1 acc).2)]
   | concat r1 r2 ih1 ih2 =>
@@ -529,17 +526,16 @@ theorem extract_replaceFrom_is_id (r: Regex σ) (acc: Symbols σ l):
       r1 =
         (replace
           (RegexID.add_concat (RegexID.add (num r2) (extract r1 acc).1))
-          (Symbols.add_concat (extract r2 (extract r1 acc).2).2)
+          (Vec.cast_concat (extract r2 (extract r1 acc).2).2)
           hr
         ) := by
       clear ih2
       rw [RegexID.add_concat]
-      rw [Symbols.add_concat]
+      rw [Vec.cast_concat]
       rw [<- replace_cast_both]
       rw [<- replace_regexid_add]
       rw [<- replace_take]
       generalize_proofs h1
-      unfold Symbols.take
       rw [extract_take]
       generalize_proofs h1 h2
       nth_rewrite 1 [ih1 acc]
@@ -549,7 +545,7 @@ theorem extract_replaceFrom_is_id (r: Regex σ) (acc: Symbols σ l):
     clear ih1
     congr
     rw [RegexID.add_concat]
-    rw [Symbols.add_concat]
+    rw [Vec.cast_concat]
     rw [<- replace_cast_both]
     rw [<- ih2 ((extract r1 acc).2)]
   | star r1 ih1 =>
@@ -558,111 +554,48 @@ theorem extract_replaceFrom_is_id (r: Regex σ) (acc: Symbols σ l):
     intro n acc hr
     rw [<- ih1 acc]
 
-theorem extract_replace_is_id (r: Regex σ) (acc: Symbols σ l):
+theorem extract_replace_is_id (r: Regex σ) (acc: Vec σ l):
   r = replace (extract r acc).1 (extract r acc).2 (by omega):= by
   rw [<- replaceFrom]
   rw [<- extract_replaceFrom_is_id]
-
-def extractFrom (r: Regex σ): RegexID (num r) × Symbols σ (num r) :=
-  match extract r List.Vector.nil with
-  | (r', xs) => (RegexID.cast r' (by omega), Symbols.cast xs (by omega))
 
 theorem extractFrom_replaceFrom_is_id (r: Regex σ):
   r = replaceFrom (extractFrom r).1 (extractFrom r).2 := by
   simp only [extractFrom]
   simp only [replaceFrom]
   rw [<- replace_cast_both]
-  rw [<- extract_replace_is_id r List.Vector.nil]
+  rw [<- extract_replace_is_id r Vec.nil]
 
 theorem nums_cons_is_add:
-  nums (⟨x::xs, h⟩)
-  = num x + nums ⟨xs, congrArg Nat.pred h⟩
+  nums (Vec.cons x xs) = num x + nums xs
   := by
-  simp [nums]
+  simp only [nums]
   ac_rfl
 
 theorem RegexID.cons_cast:
-  List.Vector (RegexID (nacc + nums (⟨x::xs, h⟩))) n
-  = List.Vector (RegexID (nacc + num x + nums ⟨xs, congrArg Nat.pred h⟩)) n := by
-  simp [nums]
+  Vec (RegexID (nacc + nums (Vec.cons x xs))) n
+  = Vec (RegexID (nacc + num x + nums xs)) n := by
+  simp only [nums]
   ac_rfl
 
-def extracts (xs: List.Vector (Regex σ) nregex) (acc: Symbols σ nacc):
-  (List.Vector (RegexID (nacc + nums xs)) nregex) × (Symbols σ (nacc + nums xs)) :=
-  match xs with
-  | ⟨[], h⟩ =>
-    (
-      ⟨[], by assumption ⟩,
-      ⟨acc.val, by simp only [List.Vector.length_val, nums, add_zero]⟩
-    )
-  | ⟨x::xs, h⟩ =>
-    let xs': List.Vector (Regex σ) nregex.pred := ⟨xs, congrArg Nat.pred h⟩
-    let (regex, symbols) := Symbol.extract x acc
-    let regex' := RegexID.add (nums ⟨xs, congrArg Nat.pred h⟩) regex
-    let regex'': RegexID (nacc + nums (⟨x::xs, h⟩)) :=
-      RegexID.cast
-      regex'
-      (by
-        simp
-        rw [nums_cons_is_add]
-        ac_rfl
-      )
-    let (regexes, symbols') := extracts xs' symbols
-    let regexes': List.Vector (RegexID (nacc + nums (⟨x::xs, h⟩))) nregex.pred
-      := by
-        rw [RegexID.cons_cast]
-        exact regexes
-    let regexes'' : List.Vector (RegexID (nacc + nums (⟨x::xs, h⟩))) nregex :=
-      (Symbols.cast
-        ((List.Vector.cons
-          regex''
-          regexes'
-        ): List.Vector (RegexID (nacc + nums (⟨x::xs, h⟩))) nregex.pred.succ)
-        (by
-          rw [<- h]
-          simp only [List.length_cons, Nat.pred_eq_sub_one, add_tsub_cancel_right, Nat.succ_eq_add_one]
-        )
-      )
-    let symbols': Symbols σ (nacc + nums (⟨x::xs, h⟩)) :=
-      Symbols.cast
-      symbols'
-      (by
-        simp [nums]
-        ac_rfl
-      )
-    (
-      regexes'',
-      symbols'
-    )
+theorem extracts_nil (acc: Vec σ nacc):
+  extracts (@Vec.nil (Regex σ)) acc = (RegexID.casts Vec.nil (by
+    simp only [nums_nil]
+    rfl
+  ), Vec.cast acc (by
+    simp only [nums_nil]
+    simp only [add_zero]
+  )) := by
+  simp only [extracts]
+  rfl
 
-def extractsSymbols (xs: List.Vector (Regex σ) l1) (acc: Symbols σ l2):
-  Symbols σ (l2 + Symbol.nums xs) :=
-  match xs with
-  | ⟨[], h⟩ => ⟨acc.val, by simp only [List.Vector.length_val, Symbol.nums, add_zero]⟩
-  | ⟨x::xs, h⟩ =>
-      (Symbol.Symbols.cast
-        (extractsSymbols ⟨xs, congrArg Nat.pred h⟩ (Symbol.extract x acc).2)
-        (by simp only [Symbol.nums]; ac_rfl)
-      )
-
-def extracts_list (xs: List (Regex σ)) (acc: List σ):
-  (List (RegexID (acc.length + nums_list xs))) × (List σ) :=
-  let (r1, r2) := extracts (Vec.fromList xs) (Vec.fromList acc)
-  let r2List: List σ := List.Vector.toList r2
-  (r1.toList, r2List)
-
-theorem snoc_fmap:
-  (List.Vector.map f (Symbols.snoc acc s))
-  = (Symbols.snoc (List.Vector.map f acc) (f s)) := by
-  simp_all only [List.Vector.map_snoc]
-
-theorem map_cast (xs: List.Vector α l1) (f: α -> β) (h: l1 = l2):
-  List.Vector.map f (Symbols.cast xs h) = Symbols.cast (List.Vector.map f xs) h := by
+theorem map_cast (xs: Vec α l1) (f: α -> β) (h: l1 = l2):
+  Vec.map (Vec.cast xs h) f = Vec.cast (Vec.map xs f) h := by
   subst h
   rfl
 
-theorem extract_replaceFrom_is_fmap (r: Regex α) (acc: Symbols α l) (f: α -> β):
-  Regex.map r f = replaceFrom (extract r acc).1 (List.Vector.map f (extract r acc).2) := by
+theorem extract_replaceFrom_is_fmap (r: Regex α) (acc: Vec α l) (f: α -> β):
+  Regex.map r f = replaceFrom (extract r acc).1 (Vec.map (extract r acc).2 f) := by
   simp only [replaceFrom]
   generalize_proofs hr
   revert acc l
@@ -676,8 +609,8 @@ theorem extract_replaceFrom_is_fmap (r: Regex α) (acc: Symbols α l) (f: α -> 
   | symbol s =>
     intro n acc hr
     simp only [replace, extract, Regex.map]
-    simp only [snoc_fmap]
-    rw [Symbols.push_get]
+    simp only [Vec.snoc_map]
+    rw [Vec.snoc_get]
   | or r1 r2 ih1 ih2 =>
     intro n acc hr
     simp only [extract]
@@ -687,18 +620,17 @@ theorem extract_replaceFrom_is_fmap (r: Regex α) (acc: Symbols α l) (f: α -> 
       Regex.map r1 f =
         (replace
           (RegexID.add_or (RegexID.add (num r2) (extract r1 acc).1))
-          (List.Vector.map f (Symbols.add_or (extract r2 (extract r1 acc).2).2))
+          (Vec.map (Vec.cast_or (extract r2 (extract r1 acc).2).2) f)
           hr
         ) := by
       clear ih2
       rw [RegexID.add_or]
-      rw [Symbols.add_or]
+      rw [Vec.cast_or]
       rw [map_cast]
       rw [<- replace_cast_both]
       rw [<- replace_regexid_add]
       rw [<- replace_take]
       generalize_proofs h1
-      unfold Symbols.take
       rw [extract_take_fmap]
       generalize_proofs h1 h2
       have ih1' := ih1 acc
@@ -709,7 +641,7 @@ theorem extract_replaceFrom_is_fmap (r: Regex α) (acc: Symbols α l) (f: α -> 
     clear ih1
     congr
     rw [RegexID.add_or]
-    rw [Symbols.add_or]
+    rw [Vec.cast_or]
     rw [map_cast]
     rw [<- replace_cast_both]
     rw [<- ih2 ((extract r1 acc).2)]
@@ -722,18 +654,17 @@ theorem extract_replaceFrom_is_fmap (r: Regex α) (acc: Symbols α l) (f: α -> 
       Regex.map r1 f =
         (replace
           (RegexID.add_concat (RegexID.add (num r2) (extract r1 acc).1))
-          (List.Vector.map f (Symbols.add_concat (extract r2 (extract r1 acc).2).2))
+          (Vec.map (Vec.cast_concat (extract r2 (extract r1 acc).2).2) f)
           hr
         ) := by
       clear ih2
       rw [RegexID.add_concat]
-      rw [Symbols.add_concat]
+      rw [Vec.cast_concat]
       rw [map_cast]
       rw [<- replace_cast_both]
       rw [<- replace_regexid_add]
       rw [<- replace_take]
       generalize_proofs h1
-      unfold Symbols.take
       rw [extract_take_fmap]
       generalize_proofs h1 h2
       have ih1' := ih1 acc
@@ -744,7 +675,7 @@ theorem extract_replaceFrom_is_fmap (r: Regex α) (acc: Symbols α l) (f: α -> 
     clear ih1
     congr
     rw [RegexID.add_concat]
-    rw [Symbols.add_concat]
+    rw [Vec.cast_concat]
     rw [map_cast]
     rw [<- replace_cast_both]
     rw [<- ih2 ((extract r1 acc).2)]
@@ -755,39 +686,18 @@ theorem extract_replaceFrom_is_fmap (r: Regex α) (acc: Symbols α l) (f: α -> 
     rw [<- ih1 acc]
     simp only [Regex.map]
 
-theorem extract_replace_is_fmap (r: Regex α) (acc: Symbols α l) (f: α -> β):
-  Regex.map r f = replace (extract r acc).1 (List.Vector.map f (extract r acc).2) (by omega) := by
+theorem extract_replace_is_fmap (r: Regex α) (acc: Vec α l) (f: α -> β):
+  Regex.map r f = replace (extract r acc).1 (Vec.map (extract r acc).2 f) (by omega) := by
   rw [<- replaceFrom]
   rw [<- extract_replaceFrom_is_fmap]
 
 theorem extractFrom_replaceFrom_is_fmap (r: Regex α) (f: α -> β):
-  Regex.map r f = replaceFrom (extractFrom r).1 (List.Vector.map f (extractFrom r).2) := by
+  Regex.map r f = replaceFrom (extractFrom r).1 (Vec.map (extractFrom r).2 f) := by
   simp only [extractFrom]
   simp only [replaceFrom]
   rw [map_cast]
   rw [<- replace_cast_both]
-  rw [<- extract_replace_is_fmap r List.Vector.nil]
-
-def derive {σ: Type} {α: Type} (p: σ -> α -> Bool) (r: Regex σ) (a: α): Regex σ :=
-  Regex.derive2 (replaceFrom (extractFrom r).1 (List.Vector.map (fun s => (s, p s a)) (extractFrom r).2))
-
-def derive' {σ: Type} {α: Type} (p: σ -> α -> Bool) (r: Regex σ) (a: α): Regex σ :=
-  let (r', symbols): (RegexID (num r) × Symbols σ (num r)) := extractFrom r
-  let pred_results: List.Vector Bool (num r) := List.Vector.map (fun s => p s a) symbols
-  let replaces: List.Vector (σ × Bool) (num r) := Vec.zip symbols pred_results
-  let replaced: Regex (σ × Bool) := replaceFrom r' replaces
-  Regex.derive2 replaced
-
-theorem zip_map {α: Type} {β: Type} (f: α -> β) (xs: List.Vector α l):
-  (List.Vector.map (fun x => (x, f x)) xs) =
-  (Vec.zip xs (List.Vector.map f xs)) := by
-  simp only [Vec.zip, List.Vector.map]
-  cases xs with
-  | mk xs h =>
-  simp only
-  congr
-  rw [← List.zip_eq_zipWith]
-  rw [← List.map_prod_left_eq_zip]
+  rw [<- extract_replace_is_fmap r Vec.nil]
 
 theorem Symbol_derive_is_derive'
   {σ: Type} {α: Type} (p: σ -> α -> Bool) (r: Regex σ) (a: α):
@@ -795,7 +705,7 @@ theorem Symbol_derive_is_derive'
   unfold Symbol.derive
   unfold Symbol.derive'
   simp only
-  rw [zip_map]
+  rw [Vec.zip_map]
 
 theorem Symbol_derive_is_Regex_derive
   {σ: Type} {α: Type} (p: σ -> α -> Bool) (r: Regex σ) (a: α):
@@ -804,57 +714,608 @@ theorem Symbol_derive_is_Regex_derive
   rw [<- extractFrom_replaceFrom_is_fmap]
   rw [Regex.derive_is_derive2]
 
-def extractsFrom (xs: List.Vector (Regex σ) nregex):
-  (List.Vector (RegexID (nums xs)) nregex) × (Symbols σ (nums xs)) :=
-  let (xs0, symbols0) := extracts xs List.Vector.nil
-  let symbols': Symbols σ (nums xs) := Symbols.cast symbols0 (by ac_rfl)
-  let xs': List.Vector (RegexID (nums xs)) nregex := RegexID.casts xs0 (by ac_rfl)
-  (xs', symbols')
+theorem RegexID.casts_rfl {n} {xs : Vec (RegexID n) l} {h : n = n} : RegexID.casts xs h = xs := by
+  induction xs with
+  | nil =>
+    unfold RegexID.casts
+    rfl
+  | @cons l x xs ih =>
+    simp only [casts] at *
+    simp only [Vec.map]
+    rw [ih]
+    rfl
 
-def replacesFrom (rs: List.Vector (RegexID n) l) (xs: List.Vector σ n): List.Vector (Regex σ) l :=
-  List.Vector.map (fun r => replaceFrom r xs) rs
-
-def derives {σ: Type} {α: Type} (p: σ -> α -> Bool) (rs: List.Vector (Regex σ) l) (a: α): List.Vector (Regex σ) l :=
-  let (rs', symbols): (List.Vector (RegexID (nums rs)) l × Symbols σ (nums rs)) := Symbol.extractsFrom rs
-  let pred_results: List.Vector Bool (nums rs) := List.Vector.map (fun s => p s a) symbols
-  let replaces: List.Vector (σ × Bool) (nums rs) := Vec.zip symbols pred_results
-  let replaced: List.Vector (Regex (σ × Bool)) l := replacesFrom rs' replaces
-  Regex.derives2 replaced
-
-theorem replacesFrom_cast_both (rs: List.Vector (RegexID n) l) (ss: Symbols σ n) (h: n = m):
+theorem replacesFrom_cast_both (rs: Vec (RegexID n) l) (ss: Vec σ n) (h: n = m):
   replacesFrom rs ss =
-  replacesFrom (RegexID.casts rs h) (Symbols.cast ss h) := by
-  sorry
+  replacesFrom (RegexID.casts rs h) (Vec.cast ss h) := by
+  subst h
+  simp only [Vec.cast_rfl]
+  simp only [RegexID.casts_rfl]
 
-theorem extractsFrom_replacesFrom_is_fmap (rs: List.Vector (Regex α) l) (f: α -> β):
-  Regexes.map rs f = replacesFrom (extractsFrom rs).1 (List.Vector.map f (extractsFrom rs).2) := by
-  unfold extractsFrom
-  simp only
-  unfold Regexes.map
-  generalize_proofs hnumrs
-  rw [map_cast]
+theorem num_map (r: Regex α) (f: α -> β):
+  num (Regex.map r f) = num r := by
+  fun_induction num with
+  | case1 =>
+    simp only [Regex.map, num]
+  | case2 =>
+    simp only [Regex.map, num]
+  | case3 =>
+    simp only [Regex.map, num]
+  | case4 r1 r2 hr1 hr2 =>
+    simp only [Regex.map, num, hr1, hr2]
+  | case5 r1 r2 hr1 hr2 =>
+    simp only [Regex.map, num, hr1, hr2]
+  | case6 r1 hr1 =>
+    simp only [Regex.map, hr1]
+
+theorem nums_map (rs: Vec (Regex α) l) (f: α -> β):
+  nums (Regexes.map rs f) = nums rs := by
+  simp only [Regexes.map]
+  induction rs with
+  | nil =>
+    simp only [Vec.map]
+    rfl
+  | @cons l r rs ih =>
+    simp only [Vec.map]
+    simp only [nums]
+    rw [ih]
+    rw [num_map]
+
+theorem extract_lift_cast (r: Regex α) (acc: Vec α n) (h1: n + num r = l + num r) (h2: n = l):
+  (Vec.cast (extract r acc).2 h1) = (extract r (Vec.cast acc h2)).2 := by
+  subst h2
+  rfl
+
+theorem extract_lift_cast_1 (r: Regex α) (acc: Vec α n) (h1: n + num r = l + num r) (h2: n = l):
+  RegexID.cast (extract r acc).1 h1 = (extract r (Vec.cast acc h2)).1 := by
+  subst h2
+  rfl
+
+theorem extract_is_fmap_2 (r: Regex α) (acc: Vec α n) (f: α -> β):
+  (extract (Regex.map r f) (Vec.map acc f)).2 = Vec.cast (Vec.map (extract r acc).2 f) (by rw [num_map]) := by
+  generalize_proofs hr
+  fun_induction extract with
+  | case1 =>
+    apply Vec.eq
+    simp only [extract, Regex.map]
+    rfl
+  | case2 =>
+    apply Vec.eq
+    simp only [extract, Regex.map]
+    rfl
+  | case3 =>
+    apply Vec.eq
+    simp only [extract, Regex.map, num]
+    rw [Vec.cast_toList]
+    rw [Vec.snoc_map]
+  | case4 acc r1 r2 er1 acc1 he1 er2 acc2 he2 ih1 ih2 => -- or
+    rename_i n
+    simp [Regex.map] at *
+    have hacc1 : acc1 = (extract r1 acc).2 := by
+      rw [he1]
+    have hacc2 : acc2 = (extract r2 (extract r1 acc).2).2 := by
+      rw [<- hacc1]
+      rw [he2]
+    rw [hacc2]
+    rw [hacc1] at ih2
+    have ih1' := ih1 (by rw [num_map])
+    clear ih1
+    have ih2' := ih2 (by rw [num_map])
+    clear ih2
+    simp only [extract]
+    simp only [Vec.cast_or]
+    rw [ih1']
+    have hh: n + num r1 + num (r2.map f) = n + num (r1.map f) + num (r2.map f) := by
+      repeat rw [num_map]
+    rw [<- extract_lift_cast (h1 := hh)]
+    rw [ih2']
+    apply Vec.eq
+    rw [map_cast]
+    repeat rw [Vec.cast_cast]
+  | case5 acc r1 r2 er1 acc1 he1 er2 acc2 he2 ih1 ih2 => -- concat
+    rename_i n
+    simp only [Regex.map] at *
+    have hacc1 : acc1 = (extract r1 acc).2 := by
+      rw [he1]
+    have hacc2 : acc2 = (extract r2 (extract r1 acc).2).2 := by
+      rw [<- hacc1]
+      rw [he2]
+    rw [hacc2]
+    rw [hacc1] at ih2
+    have ih1' := ih1 (by rw [num_map])
+    clear ih1
+    have ih2' := ih2 (by rw [num_map])
+    clear ih2
+    simp only [extract]
+    simp only [Vec.cast_concat]
+    rw [ih1']
+    have hh: n + num r1 + num (r2.map f) = n + num (r1.map f) + num (r2.map f) := by
+      repeat rw [num_map]
+    rw [<- extract_lift_cast (h1 := hh)]
+    rw [ih2']
+    apply Vec.eq
+    rw [map_cast]
+    congr 1
+    simp only [Vec.cast_cast]
+  | case6 acc r1 er1 acc1 he ih1 => -- star
+    simp only [Nat.add_left_cancel_iff, Regex.map, num] at *
+    have hacc1 : acc1 = (extract r1 acc).2 := by
+      rw [he]
+    rw [hacc1]
+    rw [<- ih1]
+    rfl
+    rw [num_map]
+
+theorem extract_is_fmap_1 (r: Regex α) (acc: Vec α n) (f: α -> β):
+  (extract (Regex.map r f) (Vec.map acc f)).1 = RegexID.cast (extract r acc).1 (by simp only [num_map]) := by
+  generalize_proofs hr
+  fun_induction extract with
+  | case1 =>
+    simp only [Regex.map, extract, RegexID.cast]
+  | case2 =>
+    simp only [Regex.map, extract, RegexID.cast]
+  | case3 =>
+    simp only [Regex.map, extract, RegexID.cast]
+  | case4 acc r1 r2 er1 acc1 he1 er2 acc2 he2 ih1 ih2 =>
+    rename_i n
+
+    have hacc1 : acc1 = (extract r1 acc).2 := by
+      rw [he1]
+    have hacc2 : acc2 = (extract r2 (extract r1 acc).2).2 := by
+      rw [<- hacc1]
+      rw [he2]
+    have her1 : er1 = (extract r1 acc).1 := by
+      rw [he1]
+    have her2 : er2 = (extract r2 (extract r1 acc).2).1 := by
+      rw [<- hacc1]
+      rw [he2]
+    rw [hacc1] at ih2
+    clear he1
+    clear he2
+
+    subst_vars
+
+    have hr1: n + num r1 = n + num (r1.map f) := by
+      rw [num_map]
+    have ih1' := ih1 hr1
+    clear ih1
+    have hr2: n + num r1 + num r2 = n + num r1 + num (r2.map f) := by
+      rw [num_map]
+    have ih2' := ih2 hr2
+    clear ih2
+
+    simp only [Regex.map]
+    simp only [extract]
+
+    rw [ih1']
+    rw [extract_is_fmap_2]
+    generalize_proofs
+    have hhlift : n + num r1 + num (r2.map f) = n + num (r1.map f) + num (r2.map f) := by
+      repeat rw [num_map]
+    have hlift := extract_lift_cast_1 (r := r2.map f) (acc := Vec.map (extract r1 acc).2 f) (h2 := hr1) (h1 := hhlift)
+    rw [<- hlift]
+    clear hlift
+    rw [ih2']
+    clear ih1'
+    clear ih2'
+
+    simp only [RegexID.add]
+    simp only [RegexID.add_or]
+    simp only [RegexID.add_assoc]
+    repeat rw [RegexID.cast_is_cast_map]
+    unfold RegexID.cast_map
+    simp only [Regex.map_map]
+    congr 1
+    · simp only [num, Fin.castLE_castLE, Regex.map_map]
+    · simp only [num, Fin.castLE_castLE, Regex.map_map]
+  | case5 acc r1 r2 er1 acc1 he1 er2 acc2 he2 ih1 ih2 =>
+    rename_i n
+
+    have hacc1 : acc1 = (extract r1 acc).2 := by
+      rw [he1]
+    have hacc2 : acc2 = (extract r2 (extract r1 acc).2).2 := by
+      rw [<- hacc1]
+      rw [he2]
+    have her1 : er1 = (extract r1 acc).1 := by
+      rw [he1]
+    have her2 : er2 = (extract r2 (extract r1 acc).2).1 := by
+      rw [<- hacc1]
+      rw [he2]
+    rw [hacc1] at ih2
+    clear he1
+    clear he2
+
+    subst_vars
+
+    have hr1: n + num r1 = n + num (r1.map f) := by
+      rw [num_map]
+    have ih1' := ih1 hr1
+    clear ih1
+    have hr2: n + num r1 + num r2 = n + num r1 + num (r2.map f) := by
+      rw [num_map]
+    have ih2' := ih2 hr2
+    clear ih2
+
+    simp only [Regex.map]
+    simp only [extract]
+
+    rw [ih1']
+    rw [extract_is_fmap_2]
+    generalize_proofs
+    have hhlift : n + num r1 + num (r2.map f) = n + num (r1.map f) + num (r2.map f) := by
+      repeat rw [num_map]
+    have hlift := extract_lift_cast_1 (r := r2.map f) (acc := Vec.map (extract r1 acc).2 f) (h2 := hr1) (h1 := hhlift)
+    rw [<- hlift]
+    rw [ih2']
+
+    simp only [RegexID.add]
+    simp only [RegexID.add_concat]
+    simp only [RegexID.add_assoc]
+    repeat rw [RegexID.cast_is_cast_map]
+    unfold RegexID.cast_map
+    simp only [Regex.map_map]
+    congr 1
+    · simp only [num, Fin.castLE_castLE, Regex.map_map]
+    · simp only [num, Fin.castLE_castLE, Regex.map_map]
+  | case6 acc r1 er1 acc1 he1 ih1 =>
+    rename_i n
+
+    have hacc1 : acc1 = (extract r1 acc).2 := by
+      rw [he1]
+    have her1 : er1 = (extract r1 acc).1 := by
+      rw [he1]
+    clear he1
+
+    subst_vars
+
+    have hr1: n + num r1 = n + num (r1.map f) := by
+      rw [num_map]
+    have ih1' := ih1 hr1
+    clear ih1
+
+    simp only [Regex.map]
+    simp only [extract]
+
+    rw [ih1']
+    generalize (extract r1 acc).1 = rid
+
+    repeat rw [RegexID.cast_is_cast_map]
+    unfold RegexID.cast_map
+    simp only [Regex.map]
+
+theorem extracts_lift_cast (rs: Vec (Regex α) m) (acc: Vec α n) (h1: n + nums rs = l + nums rs) (h2: n = l):
+  (Vec.cast (extracts rs acc).2 h1) = (extracts rs (Vec.cast acc h2)).2 := by
+  subst h2
+  rfl
+
+theorem extracts_fmap2 (rs: Vec (Regex α) l) (acc: Vec α n) (f: α -> β):
+  (Vec.map (extracts rs acc).2 f)
+  = (Vec.cast (extracts (Regexes.map rs f) (Vec.map acc f)).2 (by
+    rw [Nat.add_right_inj]
+    apply nums_map
+  )) := by
+  generalize_proofs h
+  induction rs generalizing n acc with
+  | nil =>
+    apply Vec.eq
+    simp only [Vec.toList_map]
+    simp only [Regexes.map]
+    simp only [extracts, Vec.map]
+    rw [Vec.cast_toList]
+    rw [Vec.map_toList]
+  | @cons l r rs ih =>
+    simp only [extracts]
+    have h' : n + num r + nums (Regexes.map rs f) = n + num r + nums rs := by
+      simp only [nums_map]
+    have ih' := ih ((extract r acc).2) h'
+    apply Vec.eq
+    repeat rw [Vec.toList_cast]
+    rw [Vec.map_cast]
+    rw [ih']
+    repeat rw [Vec.toList_cast]
+    simp only [Regexes.map]
+    simp only [Vec.map]
+    simp only [extracts]
+    repeat rw [Vec.toList_cast]
+    have hextract := extract_is_fmap_2 (f := f) (r := r) (n := n)
+    rw [hextract]
+    rw [<- extracts_lift_cast]
+    repeat rw [Vec.toList_cast]
+    congr 1
+    simp only [num_map]
+
+theorem RegexID.casts_symm:
+  RegexID.casts rs1 h = rs2
+  <->
+  RegexID.casts rs2 (Eq.symm h) = rs1 := by
+  apply Iff.intro
+  case mp =>
+    intro h
+    rw [<- h]
+    unfold RegexID.casts
+    rw [Vec.map_map]
+    simp only [RegexID.cast_is_cast_map]
+    unfold RegexID.cast_map
+    simp only [Regex.map_map]
+    rename_i h_1
+    subst h h_1
+    simp_all only [Fin.castLE_refl]
+    simp only [Regex.map_id]
+    simp only [Vec.map_id]
+  case mpr =>
+    intro h
+    rw [<- h]
+    unfold RegexID.casts
+    rw [Vec.map_map]
+    simp only [RegexID.cast_is_cast_map]
+    unfold RegexID.cast_map
+    simp only [Regex.map_map]
+    rename_i h_1
+    subst h h_1
+    simp_all only [Fin.castLE_refl]
+    simp only [Regex.map_id]
+    simp only [Vec.map_id]
+
+theorem extracts_append (acc: Vec α n) (xs: Vec (Regex α) l):
+  (extracts xs acc).2 = Vec.cast (Vec.append acc (extracts xs Vec.nil).2) (by omega) := by
+  induction xs generalizing acc n with
+  | nil =>
+    simp only [extracts, Vec.append_nil, Vec.cast_cast]
+    rfl
+  | @cons l x xs ih =>
+    simp only [extracts]
+    rw [ih]
+    rw [extract_append]
+    nth_rewrite 2 [ih]
+    rw [Vec.append_cast_r]
+    rw [Vec.cast_cast]
+    rw [Vec.cast_cast]
+    rw [Vec.append_cast_l]
+    rw [Vec.cast_cast]
+    rw [Vec.append_cast_r]
+    rw [Vec.cast_cast]
+    rw [Vec.append_assoc_l]
+    rw [Vec.cast_cast]
+
+theorem extracts_take (r: Regex α) (acc: Vec α n) (rs: Vec (Regex α) l):
+  (Vec.take (n + num r) (extracts rs (extract r acc).2).2)
+    = Vec.cast (extract r acc).2 (by omega) := by
+  rw [extracts_append]
+  rw [Vec.take_lift_cast]
+  rw [Vec.take_append]
+  rw [Vec.cast_cast]
+
+theorem RegexID.cast_lift_cons {x: RegexID n} {h: n = m} {xs: Vec (RegexID n) l}:
+  Vec.cons (RegexID.cast x h) (RegexID.casts xs h)
+  = RegexID.casts (Vec.cons x xs) h := by
+  simp only [RegexID.casts]
+  simp only [Vec.map]
+
+theorem RegexID.castLE_lift_cons {x: RegexID n} {h: n ≤ m} {xs: Vec (RegexID n) l}:
+  Vec.cons (RegexID.castLE x h) (RegexID.castsLE xs h)
+  = RegexID.castsLE (Vec.cons x xs) h := by
+  simp only [RegexID.castsLE]
+  simp only [Vec.map]
+
+theorem RegexID.castLE_id {h: n ≤ n}:
+  (RegexID.castLE r h) = r := by
+  simp only [RegexID.castLE]
+  simp_all only [Fin.castLE_refl]
+  simp_all only [le_refl]
+  rw [Regex.map_id]
+
+theorem RegexID.castLE_casts_lift_cons {x: RegexID n1} {h1: n1 ≤ k} {h2: n2 = k} {xs: Vec (RegexID n2) l}:
+  Vec.cons (RegexID.castLE x h1) (RegexID.casts xs h2)
+  = RegexID.castsLE (Vec.cons (RegexID.castLE x (by omega)) xs) (by omega) := by
+  simp only [RegexID.casts]
+  simp only [RegexID.cast_is_cast_map]
+  simp only [RegexID.cast_map]
+  simp only [RegexID.castsLE]
+  subst h2
+  simp_all only [Fin.castLE_refl]
+  simp only [Vec.map]
+  simp only [Regex.map_id]
+  generalize_proofs h2
+  simp only [Vec.map_id]
+  rw [RegexID.castLE_id]
+  congr
+  · induction xs with
+    | nil =>
+      simp only [Vec.map_nil]
+    | @cons l x xs ih =>
+      simp only [Vec.map]
+      rw [<- ih]
+      rw [RegexID.castLE_id]
+
+theorem replacesFrom_cons (rs: Vec (RegexID n) l) (xs: Vec σ n):
+  replacesFrom (Vec.cons r rs) xs
+  = Vec.cons (replaceFrom r xs) (replacesFrom rs xs)
+  := by
+  simp only [replacesFrom]
+  simp only [Vec.map]
+
+theorem RegexID.add_zero:
+  (RegexID.add 0 r) = r := by
+  simp only [Nat.add_zero, RegexID.add]
+  simp_all only [Fin.castLE_refl]
+  simp only [Regex.map_id]
+
+theorem replaceFrom_append {r: Regex α} {xs: Vec α (n + num r)} {acc: Vec α n} {ys: Vec α m}:
+  replaceFrom (RegexID.add m (extract r acc).1) (Vec.append xs ys)
+  = replaceFrom (extract r acc).1 xs := by
+  unfold replaceFrom
+  rw [← replace_regexid_add (extract r acc).1 (xs.append ys)]
+  rw [← replace_take (extract r acc).1 (xs.append ys)]
+  rw [Vec.take_append xs ys]
+  rw [replace_cast_symbols]
+
+theorem replaceFrom_extracts_cons:
+  replaceFrom (RegexID.add (nums rs) (extract r acc).1) (((extract r acc).2.append ((extracts rs Vec.nil).2.cast h)))
+  = replaceFrom (extract r acc).1 (extract r acc).2
+  := by
+  rw [replaceFrom_append]
+
+theorem extracts_replacesFrom_is_id (rs: Vec (Regex α) l) (acc: Vec α n):
+  rs = replacesFrom (extracts rs acc).1 (extracts rs acc).2 := by
+  induction rs generalizing n acc with
+  | nil =>
+    apply Vec.eq
+    simp only [extracts, replacesFrom]
+    simp only [Vec.map_nil]
+  | @cons l r rs ih =>
+    simp only [extracts]
+    rw [Vec.cast_rfl]
+    simp only [RegexID.cast_lift_cons]
+    rw [<- replacesFrom_cast_both]
+    rw [replacesFrom_cons]
+    nth_rewrite 1 [extracts_append]
+    congr 1
+    · rw [<- Vec.append_cast_r (xs := (extract r acc).2) (ys := (extracts rs Vec.nil).2) (h := (by simp only [zero_add]))]
+      rw [replaceFrom_extracts_cons]
+      rw [<- extract_replaceFrom_is_id]
+    · generalize (extract r acc).2 = acc'
+      rw [<- ih]
+
+theorem RegexID.casts_casts (xs: Vec (RegexID n1) l) (h12: n1 = n2) (h23: n2 = n3):
+  RegexID.casts (RegexID.casts xs h12) h23 = RegexID.casts xs (by omega) := by
+  subst h12 h23
+  simp only [RegexID.casts_rfl]
+
+theorem nums_map_map:
+  nums rs = nums (rs.map fun r => r.map f) := by
+  induction rs with
+  | nil =>
+    simp only [Vec.map]
+    rfl
+  | @cons l r rs ih =>
+    simp only [Vec.map]
+    simp only [nums]
+    rw [ih]
+    rw [num_map]
+
+theorem RegexID.add_cast_is_castLE (r: RegexID n) (h: n = m):
+  (RegexID.add k (RegexID.cast r h)) = RegexID.castLE r (by omega) := by
+  simp only [RegexID.add, RegexID.cast]
+  subst h
+  simp_all only
+  rfl
+
+theorem RegexID.add_is_castLE (r: RegexID n):
+  (RegexID.add k r) = RegexID.castLE r (by omega) := by
+  simp only [RegexID.add, RegexID.castLE]
+
+theorem RegexID.casts_is_casts_rw:
+  RegexID.casts xs h =
+  RegexID.casts_rw xs h := by
+  subst h
+  simp only [RegexID.casts]
+  simp only [RegexID.cast]
+  simp only [RegexID.casts_rw]
+  rw [Vec.map_id]
+
+theorem extracts_fmap1 (rs: Vec (Regex α) l) (acc: Vec α n) (f: α -> β):
+  (extracts rs acc).1
+  = (RegexID.casts (extracts (Regexes.map rs f) (Vec.map acc f)).1 (by simp only [nums_map])) := by
+  simp only [Regexes.map]
+  generalize_proofs h
+  rw [RegexID.casts_symm.mpr]
+  induction rs generalizing n acc f with
+  | nil =>
+    rw [extracts_nil]
+    simp only [RegexID.casts]
+    simp only [Vec.map_nil]
+    simp only [Vec.map]
+    rw [extracts_nil]
+    simp only [RegexID.casts]
+    simp only [Vec.map]
+  | @cons l r rs ih =>
+    simp only [Vec.map]
+    simp only [extracts]
+    generalize_proofs h1 h2 h3 h4
+    simp only [RegexID.cast_lift_cons]
+    rw [Vec.cast_rfl]
+    rw [RegexID.casts_casts]
+    generalize_proofs h5
+    clear h1 h3
+
+    rw [extract_is_fmap_2]
+    generalize_proofs h7
+
+    rw [extract_is_fmap_1]
+    generalize_proofs h8
+    clear h
+    simp only [Vec.cast_rfl]
+    clear h2
+
+    simp only [<- Vec.map_cast]
+
+    have ih' : n + num (r.map f) + nums (rs.map fun r => r.map f) = n + num (r.map f) + nums rs := by
+      simp only [Nat.add_left_cancel_iff]
+      rw [<- nums_map_map]
+    rw [<- ih (h := ih')]
+    clear ih
+    generalize_proofs h9
+    clear ih'
+
+    rw [RegexID.add_cast_is_castLE]
+    generalize_proofs h10
+    simp only [RegexID.add_is_castLE]
+    generalize_proofs h11
+
+    congr 1
+    · simp_all only [Nat.add_left_cancel_iff, add_le_add_iff_left] -- aesop
+    · congr 1
+      · simp_all only [Nat.add_left_cancel_iff, add_le_add_iff_left] -- aesop
+      · congr 1
+        · simp_all only [Nat.add_left_cancel_iff, add_le_add_iff_left] -- aesop
+        · simp_all only [Nat.add_left_cancel_iff, add_le_add_iff_left, heq_eq_eq] -- aesop
+      · simp only [RegexID.casts_is_casts_rw]
+        simp only [RegexID.casts_rw]
+        simp only [Vec.cast]
+        simp_all only [add_le_add_iff_left, heq_eqRec_iff_heq]
+        simp_all only
+        congr 1
+        · simp_all only [Nat.add_left_cancel_iff] -- aesop
+        · simp_all only [Nat.add_left_cancel_iff] -- aesop
+        · congr 1
+          · simp_all only [heq_eqRec_iff_heq, heq_eq_eq] -- aesop
+    · simp_all only [Nat.add_left_cancel_iff, add_le_add_iff_left, heq_eq_eq] -- aesop
+
+theorem extracts_replacesFrom_is_fmap (rs: Vec (Regex α) l) (f: α -> β):
+  Regexes.map rs f = replacesFrom (extracts rs acc).1 (Vec.map (extracts rs acc).2 f) := by
+  rw [extracts_fmap2]
+  have hh := extracts_replacesFrom_is_id (rs := Regexes.map rs f) (acc := Vec.map acc f)
+  simp_all only
+  nth_rewrite 2 [extracts_fmap1]
   rw [<- replacesFrom_cast_both]
-  sorry
+
+theorem extractsFrom_replacesFrom_is_fmap (rs: Vec (Regex α) l) (f: α -> β):
+  Regexes.map rs f = replacesFrom (extractsFrom rs).1 (Vec.map (extractsFrom rs).2 f) := by
+  simp only [extractsFrom]
+  generalize_proofs h
+  rw [extracts_replacesFrom_is_fmap (acc := Vec.nil) (f := f)]
+  rw [replacesFrom_cast_both (h := h)]
+  simp only [map_cast]
 
 theorem Symbol_derives_is_fmap
-  {σ: Type} {α: Type} (p: σ -> α -> Bool) (rs: List.Vector (Regex σ) l) (a: α):
-  Symbol.derives p rs a = List.Vector.map (fun r => Symbol.derive p r a) rs := by
+  {σ: Type} {α: Type} (p: σ -> α -> Bool) (rs: Vec (Regex σ) l) (a: α):
+  Symbol.derives p rs a = Vec.map rs (fun r => Symbol.derive p r a) := by
   unfold Symbol.derives
   simp only
   unfold Regex.derives2
   unfold Symbol.derive
-  nth_rewrite 2 [<- List.Vector.map_map]
-  nth_rewrite 1 [<- List.Vector.map_map]
-  apply (congrArg (List.Vector.map Regex.derive2))
-  rw [<- zip_map]
+  nth_rewrite 2 [<- Vec.map_map]
+  nth_rewrite 1 [<- Vec.map_map]
+  apply (congrArg (fun xs => Vec.map xs Regex.derive2))
+  rw [<- Vec.zip_map]
   -- rewrites under the closure
   simp only [<- extractFrom_replaceFrom_is_fmap]
   rw [<- extractsFrom_replacesFrom_is_fmap]
   unfold Regexes.map
-  simp only [List.Vector.map_map]
+  simp only [Vec.map_map]
 
 theorem Symbol_derives_is_Regex_derives
-  {σ: Type} {α: Type} (p: σ -> α -> Bool) (r: List.Vector (Regex σ) l) (a: α):
+  {σ: Type} {α: Type} (p: σ -> α -> Bool) (r: Vec (Regex σ) l) (a: α):
   Symbol.derives p r a = Regex.derives p r a := by
   rw [Symbol_derives_is_fmap]
   unfold Symbol.derive
@@ -864,29 +1325,9 @@ theorem Symbol_derives_is_Regex_derives
   rw [<- extractFrom_replaceFrom_is_fmap]
   rw [Regex.derive_is_derive2]
 
-def leave
-  (rs: List.Vector (Regex σ) l)
-  (ns: List.Vector Bool (Symbol.nums rs))
-  : (List.Vector (Regex σ) l) :=
-  let replaces: List.Vector (σ × Bool) (nums rs) := Vec.zip (Symbol.extractsFrom rs).2 ns
-  let replaced: List.Vector (Regex (σ × Bool)) l := replacesFrom (Symbol.extractsFrom rs).1 replaces
-  Regex.derives2 replaced
-
-def enter (rs: List.Vector (Regex σ) l): Symbols σ (nums rs) :=
-  let (_, symbols): (List.Vector (RegexID (nums rs)) l × Symbols σ (nums rs)) := Symbol.extractsFrom rs
-  symbols
-
--- derives_preds unlike derives takes a predicate that works out the full vector of predicates.
--- This gives the predicate control over the evaluation order of α, for example α is a tree, we can first evaluate the same label, before traversing down.
-def derives_preds {σ: Type} {α: Type}
-  (ps: {n: Nat} -> List.Vector σ n -> α -> List.Vector Bool n) (rs: List.Vector (Regex σ) l) (a: α): List.Vector (Regex σ) l :=
-  let symbols: Symbols σ (nums rs) := enter rs
-  let pred_results: List.Vector Bool (nums rs) := ps symbols a
-  leave rs pred_results
-
 theorem Symbol_derive_is_derive_preds
-  {σ: Type} {α: Type} (ps: {n: Nat} -> List.Vector σ n -> α -> List.Vector Bool n) (rs: List.Vector (Regex σ) l) (a: α)
-  (h: ∀ {n': Nat} (xs: List.Vector σ n') (a: α), ps xs a = List.Vector.map (fun x => (ps (Vec.singleton x) a).head) xs):
+  {σ: Type} {α: Type} (ps: {n: Nat} -> Vec σ n -> α -> Vec Bool n) (rs: Vec (Regex σ) l) (a: α)
+  (h: ∀ {n': Nat} (xs: Vec σ n') (a: α), ps xs a = Vec.map xs (fun x => (ps (Vec.singleton x) a).head)):
   Symbol.derives (fun s a => (ps (Vec.singleton s) a).head) rs a = Symbol.derives_preds ps rs a := by
   unfold derives
   simp only
