Validator/Derive/Enter.lean
@@ -8,9 +8,9 @@ import Validator.Expr.Symbol
 namespace Enter
 
 def deriveEnter (xs: Rules n (Pred α) l): IfExprs n α (Symbol.nums xs) :=
-  List.Vector.map
-    (fun (pred, ref) => IfExpr.mk pred ref)
+  Vec.map
     (Symbol.extractsFrom xs).2
+    (fun (pred, ref) => IfExpr.mk pred ref)
 
 class DeriveEnter (m: Type -> Type u) (n: Nat) (α: outParam Type) where
   deriveEnter {l: Nat} (xs: Rules n (Pred α) l): m (IfExprs n α (Symbol.nums xs))
