Validator/Learning/Parser.lean
@@ -2,6 +2,9 @@
 -- This version of the algorithm uses a Parser instead of a Hedge.Node.
 -- It is intended to be used for explanation purposes. This means that it gives up speed for readability. Thus it has no memoization implemented.
 
+import Validator.Std.Hedge
+import Validator.Std.Vec
+
 import Validator.Expr.Compress
 import Validator.Expr.Grammar
 import Validator.Expr.IfExpr
@@ -9,7 +12,6 @@ import Validator.Expr.Regex
 
 import Validator.Parser.Hint
 import Validator.Parser.Parser
-import Validator.Std.Hedge
 import Validator.Parser.TokenTree
 
 import Validator.Derive.Enter
@@ -26,7 +28,7 @@ def deriveEnter [DecidableEq α] [ValidateM m n α] (g: Grammar n (Pred α)) (xs
   return IfExpr.evals g enters token
 
 def deriveLeaveM [DecidableEq α] [ValidateM m n α] (xs: Rules n (Pred α) l) (cs: Rules n (Pred α) (Symbol.nums xs)): m (Rules n (Pred α) l) :=
-  Leave.DeriveLeaveM.deriveLeaveM xs (List.Vector.map Rule.nullable cs)
+  Leave.DeriveLeaveM.deriveLeaveM xs (Vec.map cs Rule.nullable)
 
 def deriveValue [DecidableEq α] [ValidateM m n α] (g: Grammar n (Pred α)) (xs: Rules n (Pred α) l): m (Rules n (Pred α) l) := do
   deriveEnter g xs >>= deriveLeaveM xs
@@ -53,7 +55,7 @@ partial def derive [DecidableEq α] [ValidateM m n α] (g: Grammar n (Pred α)) 
   | Hint.eof => return xs -- only happens at the top
 
 def validate {m} [DecidableEq α] [ValidateM m n α] (g: Grammar n (Pred α)) (x: Rule n (Pred α)): m Bool := do
-  let dxs <- derive g (List.Vector.cons x List.Vector.nil)
+  let dxs <- derive g (Vec.cons x Vec.nil)
   return Rule.nullable dxs.head
 
 def run [DecidableEq α] (g: Grammar n (Pred α)) (t: Hedge.Node α): Except String Bool :=
@@ -71,7 +73,7 @@ open TokenTree (node)
 #guard run
   (Grammar.mk (n := 1)
     (Regex.symbol (Pred.eq (Token.string "a"), 0))
-    #v[Regex.emptystr]
+    #vec[Regex.emptystr]
   )
   (node "a" []) =
   Except.ok true
@@ -79,7 +81,7 @@ open TokenTree (node)
 #guard run
   (Grammar.mk (n := 1)
     (Regex.symbol (Pred.eq (Token.string "a"), 0))
-    #v[Regex.emptystr]
+    #vec[Regex.emptystr]
   )
   (node "a" [node "b" []]) =
   Except.ok false
@@ -87,7 +89,7 @@ open TokenTree (node)
 #guard run
   (Grammar.mk (n := 2)
     (Regex.symbol (Pred.eq (Token.string "a"), 0))
-    #v[
+    #vec[
       (Regex.symbol (Pred.eq (Token.string "b"), 1))
       , Regex.emptystr
     ]
@@ -98,7 +100,7 @@ open TokenTree (node)
 #guard run
   (Grammar.mk (n := 2)
     (Regex.symbol (Pred.eq (Token.string "a"), 0))
-    #v[
+    #vec[
       (Regex.concat
         (Regex.symbol (Pred.eq (Token.string "b"), 1))
         (Regex.symbol (Pred.eq (Token.string "c"), 1))
@@ -112,7 +114,7 @@ open TokenTree (node)
 #guard run
   (Grammar.mk (n := 3)
     (Regex.symbol (Pred.eq (Token.string "a"), 0))
-    #v[
+    #vec[
       (Regex.concat
         (Regex.symbol (Pred.eq (Token.string "b"), 1))
         (Regex.symbol (Pred.eq (Token.string "c"), 2))
@@ -128,7 +130,7 @@ open TokenTree (node)
 #guard run
   (Grammar.mk (n := 1)
     (Regex.symbol (Pred.eq (Token.string "a"), 0))
-    #v[Regex.emptyset]
+    #vec[Regex.emptyset]
   )
   (node "a" [node "b" []])
   = Except.ok false
@@ -136,7 +138,7 @@ open TokenTree (node)
 #guard run
   (Grammar.mk (n := 4)
     (Regex.symbol (Pred.eq (Token.string "a"), 0))
-    #v[
+    #vec[
       (Regex.concat
         (Regex.symbol (Pred.eq (Token.string "b"), 3))
         (Regex.symbol (Pred.eq (Token.string "c"), 2))
@@ -152,7 +154,7 @@ open TokenTree (node)
 #guard run
   (Grammar.mk (n := 2)
     (Regex.symbol (Pred.eq (Token.string "a"), 0))
-    #v[
+    #vec[
       (Regex.concat
         (Regex.symbol (Pred.eq (Token.string "b"), 1))
         Regex.emptyset
@@ -166,7 +168,7 @@ open TokenTree (node)
 #guard run
   (Grammar.mk (n := 3)
     (Regex.symbol (Pred.eq (Token.string "a"), 0))
-    #v[
+    #vec[
       (Regex.concat
         (Regex.symbol (Pred.eq (Token.string "b"), 1))
         (Regex.symbol (Pred.eq (Token.string "c"), 2))
@@ -181,7 +183,7 @@ open TokenTree (node)
 #guard run
   (Grammar.mk (n := 4)
     (Regex.symbol (Pred.eq (Token.string "a"), 0))
-    #v[
+    #vec[
       (Regex.concat
         (Regex.symbol (Pred.eq (Token.string "b"), 0))
         (Regex.symbol (Pred.eq (Token.string "c"), 1))
