Validator/Validator/TestMem.lean
@@ -1,4 +1,6 @@
 import Validator.Std.Hedge
+import Validator.Std.Vec
+
 import Validator.Parser.TokenTree
 
 import Validator.Validator.Validate
@@ -41,7 +43,7 @@ open TokenTree (node)
 #guard testCacheIsHitOnSecondRun
   (Grammar.mk (n := 1)
     (Regex.symbol (Pred.eq (Token.string "a"), 0))
-    #v[Regex.emptystr]
+    #vec[Regex.emptystr]
   )
   (node "a" [node "b" [], node "c" [node "d" []]])
   = Except.ok false
@@ -49,7 +51,7 @@ open TokenTree (node)
 #guard testCacheIsHitOnSecondRun
   (Grammar.mk (n := 1)
     (Regex.symbol (Pred.eq (Token.string "a"), 0))
-    #v[Regex.emptystr]
+    #vec[Regex.emptystr]
   )
   (node "a" [])
   = Except.ok true
@@ -57,7 +59,7 @@ open TokenTree (node)
 #guard testThatTestCacheBreaksWithEmptyCache
   (Grammar.mk (n := 1)
     (Regex.symbol (Pred.eq (Token.string "a"), 0))
-    #v[Regex.emptystr]
+    #vec[Regex.emptystr]
   )
   (node "a" [])
   = Except.error "test cache miss"
@@ -65,7 +67,7 @@ open TokenTree (node)
 #guard testCacheIsHitOnSecondRun
   (Grammar.mk (n := 1)
     (Regex.symbol (Pred.eq (Token.string "a"), 0))
-    #v[Regex.emptystr]
+    #vec[Regex.emptystr]
   )
   (node "a" [node "b" []])
   = Except.ok false
@@ -73,7 +75,7 @@ open TokenTree (node)
 #guard testCacheIsHitOnSecondRun
   (Grammar.mk (n := 2)
     (Regex.symbol (Pred.eq (Token.string "a"), 0))
-    #v[
+    #vec[
       (Regex.symbol (Pred.eq (Token.string "b"), 1))
       , Regex.emptystr
     ]
@@ -84,7 +86,7 @@ open TokenTree (node)
 #guard testCacheIsHitOnSecondRun
   (Grammar.mk (n := 2)
     (Regex.symbol (Pred.eq (Token.string "a"), 0))
-    #v[
+    #vec[
       (Regex.concat
         (Regex.symbol (Pred.eq (Token.string "b"), 1))
         (Regex.symbol (Pred.eq (Token.string "c"), 1))
@@ -98,7 +100,7 @@ open TokenTree (node)
 #guard testCacheIsHitOnSecondRun
   (Grammar.mk (n := 3)
     (Regex.symbol (Pred.eq (Token.string "a"), 0))
-    #v[
+    #vec[
       (Regex.concat
         (Regex.symbol (Pred.eq (Token.string "b"), 1))
         (Regex.symbol (Pred.eq (Token.string "c"), 2))
@@ -114,7 +116,7 @@ open TokenTree (node)
 #guard testCacheIsHitOnSecondRun
   (Grammar.mk (n := 1)
     (Regex.symbol (Pred.eq (Token.string "a"), 0))
-    #v[Regex.emptyset]
+    #vec[Regex.emptyset]
   )
   (node "a" [node "b" []])
   = Except.ok false
@@ -122,7 +124,7 @@ open TokenTree (node)
 #guard testCacheIsHitOnSecondRun
   (Grammar.mk (n := 4)
     (Regex.symbol (Pred.eq (Token.string "a"), 0))
-    #v[
+    #vec[
       (Regex.concat
         (Regex.symbol (Pred.eq (Token.string "b"), 3))
         (Regex.symbol (Pred.eq (Token.string "c"), 2))
@@ -138,7 +140,7 @@ open TokenTree (node)
 #guard testCacheIsHitOnSecondRun
   (Grammar.mk (n := 2)
     (Regex.symbol (Pred.eq (Token.string "a"), 0))
-    #v[
+    #vec[
       (Regex.concat
         (Regex.symbol (Pred.eq (Token.string "b"), 1))
         Regex.emptyset
@@ -152,7 +154,7 @@ open TokenTree (node)
 #guard testCacheIsHitOnSecondRun
   (Grammar.mk (n := 3)
     (Regex.symbol (Pred.eq (Token.string "a"), 0))
-    #v[
+    #vec[
       (Regex.concat
         (Regex.symbol (Pred.eq (Token.string "b"), 1))
         (Regex.symbol (Pred.eq (Token.string "c"), 2))
@@ -167,7 +169,7 @@ open TokenTree (node)
 #guard testCacheIsHitOnSecondRun
   (Grammar.mk (n := 4)
     (Regex.symbol (Pred.eq (Token.string "a"), 0))
-    #v[
+    #vec[
       (Regex.concat
         (Regex.symbol (Pred.eq (Token.string "b"), 0))
         (Regex.symbol (Pred.eq (Token.string "c"), 1))
